Reorganisation and Proved Lemma 2

proofs/LabeledGraphSemantics.thy
@@ -1,22 +1,51 @@
 theory LabeledGraphSemantics
-imports RulesAndChains
+imports LabeledGraphs
 begin
-(* gets the top relation-label as argument *)
-definition top_rule :: "'l \<Rightarrow> ('l,'v::{one,zero,numeral}) Graph_PreRule" where
-"top_rule t = (LG {} {0,1},LG {(t,0,1)} {0,1})"
-
-definition nonempty_rule :: "('l,'v::{one,zero,numeral}) Graph_PreRule" where
-"nonempty_rule = (LG {} {},LG {} {0})"
-
-(* gets a reflexive relation-label as argument *)
-definition reflexivity_rule :: "'l \<Rightarrow> ('l,'v::{one,zero,numeral}) Graph_PreRule" where
-"reflexivity_rule t = (LG {} {0},LG {(t,0,0)} {0})"
-
-(* TODO: Show they're all rules *)
-
 
 definition getRel where
 "getRel l G = {(x,y). (l,x,y) \<in> edges G}"
+
+(* Deviating from the paper in having a constant constructor.
+   We'll use that constructor for top, bottom, etc.. *)
+datatype 'v allegorical_term
+ = A_Int "'v allegorical_term" "'v allegorical_term"
+ | A_Cmp "'v allegorical_term" "'v allegorical_term"
+ | A_Cnv "'v allegorical_term"
+ | A_Lbl 'v
+
+datatype 'v Standard_Constant = S_Top | S_Bot | S_Idt | S_Const 'v
+
+abbreviation "a_bot \<equiv> A_Lbl S_Bot"
+abbreviation "a_top \<equiv> A_Lbl S_Top"
+notation a_bot ("\<bottom>")
+notation a_top ("\<top>")
+
+fun semantics where
+"semantics G (A_Int a b) = semantics G a \<inter> semantics G b" |
+"semantics G (A_Cmp a b) = semantics G a O semantics G b" |
+"semantics G (A_Cnv a) = converse (semantics G a)" |
+"semantics G (A_Lbl l) = getRel l G"
+
+notation semantics (":_:\<lbrakk>_\<rbrakk>" 55)
+
+type_synonym 'v sentence = "'v allegorical_term \<times> 'v allegorical_term"
+type_synonym 'v std_term = "'v Standard_Constant allegorical_term"
+type_synonym 'v std_sentence = "'v std_term \<times> 'v std_term"
+type_synonym 'v std_graph = "('v Standard_Constant, 'v Standard_Constant) labeled_graph"
+
+abbreviation holds where
+"holds G S \<equiv> :G:\<lbrakk>fst S\<rbrakk> = :G:\<lbrakk>snd S\<rbrakk>"
+notation holds (infix "\<tturnstile>" 55)
+
+abbreviation subset_sentence where
+"subset_sentence A B \<equiv> (A,A_Int A B)"
+
+notation subset_sentence (infix "\<sqsubseteq>" 60)
+
+lemma sentence_iff: (* Lemma 1 *)
+  "G \<tturnstile> e\<^sub>1 \<sqsubseteq> e\<^sub>2 = (:G:\<lbrakk>e\<^sub>1\<rbrakk> \<subseteq> :G:\<lbrakk>e\<^sub>2\<rbrakk>)"
+  "G \<tturnstile> (e\<^sub>1, e\<^sub>2) = (G \<tturnstile> e\<^sub>1 \<sqsubseteq> e\<^sub>2 \<and> G \<tturnstile> e\<^sub>2 \<sqsubseteq> e\<^sub>1)"
+  by auto
 
 definition standard :: "'l set \<Rightarrow> 'l \<Rightarrow> 'l \<Rightarrow> 'l \<Rightarrow> ('l, 'l) labeled_graph \<Rightarrow> bool" where
 "standard C b t idt G
@@ -27,6 +56,29 @@ definition standard :: "'l set \<Rightarrow> 'l \<Rightarrow> 'l \<Rightarrow> '
    \<and> getRel t G = {(x,y). x\<in>vertices G \<and> y\<in>vertices G}
    \<and> (\<forall> c \<in> C. getRel c G = {(c,c)})"
 
-(* Work towards Lemma 2, 6 and 7 *)
+abbreviation standard' :: "'a std_graph \<Rightarrow> bool" where
+"standard' \<equiv> standard (S_Const ` UNIV) S_Bot S_Top S_Idt"
+
+definition model :: "'a std_graph \<Rightarrow> ('a std_sentence) set \<Rightarrow> bool" where
+"model G T \<equiv> standard' G \<and> (\<forall> S \<in> T. G \<tturnstile> S)"
+notation model (infix "\<tturnstile>\<^sub>S" 55) (* S for standard *)
+
+abbreviation consistent :: "('a std_sentence) set \<Rightarrow> bool" where
+"consistent T \<equiv> \<exists> G. model G T"
+
+definition entails where
+"entails T S \<equiv> \<forall> G. G \<tturnstile>\<^sub>S T \<longrightarrow> G \<tturnstile> S"
+
+lemma standard_top_not_bot[intro]:
+"standard' G \<Longrightarrow> :G:\<lbrakk>\<bottom>\<rbrakk> \<noteq> :G:\<lbrakk>\<top>\<rbrakk>"
+  unfolding standard_def by auto
+
+lemma consistent_iff_entails_nonsense: (* Lemma 2 *)
+"consistent T = (\<not> entails T (\<bottom>,\<top>))"
+proof
+  show "consistent T \<Longrightarrow> \<not> entails T (\<bottom>, \<top>)"
+    using standard_top_not_bot unfolding entails_def model_def
+    by fastforce
+qed (auto simp:entails_def model_def)
 
 end
