proofs/RuleSemanticsConnection.thy
@@ -1,0 +1,25 @@
+theory RuleSemanticsConnection
+imports LabeledGraphSemantics RulesAndChains
+begin
+
+(* gets the top relation-label as argument *)
+definition top_rule :: "'l \<Rightarrow> ('l,'v::{one,zero,numeral}) Graph_PreRule" where
+"top_rule t = (LG {} {0,1},LG {(t,0,1)} {0,1})"
+
+definition nonempty_rule :: "('l,'v::{one,zero,numeral}) Graph_PreRule" where
+"nonempty_rule = (LG {} {},LG {} {0})"
+
+(* gets a reflexive relation-label as argument *)
+definition reflexivity_rule :: "'l \<Rightarrow> ('l,'v::{one,zero,numeral}) Graph_PreRule" where
+"reflexivity_rule t = (LG {} {0},LG {(t,0,0)} {0})"
+
+lemma are_rules[intro]:
+"graph_rule nonempty_rule"
+"graph_rule (top_rule t)"
+"graph_rule (reflexivity_rule i)"
+  unfolding reflexivity_rule_def top_rule_def nonempty_rule_def is_graph_homomorphism_def
+  by auto
+
+
+(* Work towards Lemma 5 to 7 *)
+end
